%Document Style
\documentclass[letterpaper, 12pt]{article}
\usepackage[utf8]{inputenc}
\pagestyle{empty}
\usepackage[UKenglish]{babel}
%Title Format
\usepackage{titlesec}
\titleformat{\section}{\Large\sc\raggedright}{}{0em}{}[\titlerule]
\titlespacing{\section}{0pt}{3pt}{3pt}
%Margin
\usepackage[left=1.25in,right=1.25in,top=1.25in,bottom=1.25in]{geometry}
%Font
\usepackage{amsmath, amssymb, mathptmx}
%URL
\usepackage{hyperref}
\hypersetup{pdfauthor={Takuma Kume}}
%Indent and paragraph line break
\setlength{\parindent}{0em}
\setlength{\parskip}{1em}

%%%%%%%%%%%%%%%%%%%%%%%%%%%%%%%%%%%%%%%%%%%%%%%%%%%%%%%%%%%%%%%%%%%%%%%%%%%%%%%%
\begin{document}
\underline{Tetra-molecular Self-Complementary}  $nA \leftrightarrow A_n$
\begin{align}
	G &= -RT \ln K \label{eq1}\\
	G &= \Delta H - T\Delta S \\
	\therefore \Delta H &- T \Delta S = - RT \ln K \label{htsrtlnk}
\end{align}
At $ T_m $,
\begin{align}
	\Delta H - T_m \Delta S &= - RT_m \ln K_{T_m}\\
	T_m \Delta S &= \Delta H +RT_m\ln K_{T_m}\\
	\Delta S &= \frac{\Delta H}{T_m}+R\ln K_{T_m}
\end{align}
Substitute $ \Delta S $ to equation \ref{htsrtlnk},
\begin{align}
	\Delta H - T(\frac{\Delta H}{T_m}+R\ln K_{T_m}) = - RT \ln K
\end{align}
Divide both sides by $ -RT $,
\begin{align}
	\ln K &= -\frac{\Delta H}{RT} + \frac{\Delta H}{RT_m} - \ln K_{T_m}\\
	K &= K_{T_m} e^{\frac{\Delta H}{R}\left(\frac{1}{T_m}-\frac{1}{T}\right)} \\
	\frac{K}{K_{T_m}} &= e^{\frac{\Delta H}{R}\left(\frac{1}{T_m}-\frac{1}{T}\right)}\label{kk}
\end{align}

From [Marky and Breslauer 1987], assuming at $ T_m $ $\alpha = 1/2$, association equilibrium constant K for Self-complementary sequence are,
\begin{align}
	K &= \frac{\alpha}{nC_{T}^{n-1}(1-\alpha)^n}\\
	K_{T_m} &= \frac{1}{n(C_T/2)^{n-1}}
\end{align}
Thus when $ n = 4 $ for tetra-molecular associations,
\begin{align}
	K &= \frac{\alpha}{4 C_{T}^{3}(1-\alpha)^4} \label{K4}\\
	K_{T_m} &= \frac{1}{4(C_T/2)^3} = \frac{2}{C_T^3} \label{K4Tm}\\
	\frac{K}{K_{T_m}} &= \frac{\alpha}{8\left(1-\alpha\right)^4} \qquad\text{(Association)}\label{ass}\\
	& = \frac{8\left(1-\alpha\right)^4}{\alpha} \qquad\text{(Dissociation)}\label{diss}
\end{align}
Substitute equation \ref{ass} or \ref{diss} to equation \ref{kk},
\begin{align}
	e^{\frac{\Delta H}{R}\left(\frac{1}{T_m}-\frac{1}{T}\right)} = \frac{8\left(1-\alpha\right)^4}{\alpha}
\end{align}
Solve for $\alpha$,\\
where $  x = e^{\frac{\Delta H}{R}\left(\frac{1}{T_m}-\frac{1}{T}\right)}$\\
let $ u_1 = \sqrt[3]{9x^2 + \sqrt{3}\sqrt{27x^4+2048x^3}} $\\
let $ u_2 = \sqrt[3]{18} $\\
let $ u_3 = \sqrt[3]{\frac{2}{3}}x $
%\begin{align}
%	\text{where } x &= e^{\frac{\Delta H}{R}\left(\frac{1}{T_m}-\frac{1}{T}\right)}\\
%	\text{let } u_1 &= \sqrt[3]{9x^2 + \sqrt{3}\sqrt{27x^4+2048x^3}}\\
%	\text{let } u_2 &= \sqrt[3]{18}\\
%	\text{let } u_3 &= \sqrt[3]{\frac{2}{3}} \\
%\end{align}
\begin{align}
	\alpha = \pm \frac{1}{4}\sqrt{\left(\frac{u_1}{u_2}-\frac{8u_3}{u_1}\right)}\pm \frac{1}{2}\sqrt{\left(\frac{2u_3}{u_1}+\frac{x}{2\sqrt{\frac{u_1}{u_2}-\frac{8u_3}{u_1}}}-\frac{u_1}{4u_2}\right)}+1
\end{align}
Signs are probably +,- or -,+ for each $\pm$ respectively to get physical values.

To normalise the $\alpha$ use the relation,
\begin{align}
	\frac{A_b - (N + aT)}{(D+bT)-(N+aT)}
\end{align}
where $ A_b $ is the absorbance or y-value, N and D are y-intercepts, and $ a $ and $ b $ are slopes of the flat region. Thus,
\begin{align}
	A_b = N + aT + ((b-a)T+D-N)\alpha
\end{align}

$ \divideontimes $ Temperature are in Kelvins
\end{document}